# Chapter 3: Church Numerals: Increment


## Church Numerals

The most important data in computer programs are integers.

Let's define natural integers.

$$
0=\lambda s.\lambda z.z\\
1=\lambda s.\lambda z.s(z)\\
2=\lambda s.\lambda z.s(s(z))\\
3=\lambda s.\lambda z.s(s(s(z)))\\
\vdots\\
n=\lambda s.\lambda z.s^n(z)
$$

Why should we define integers like this? What does $s$ and $z$ mean here?

Let's take $2$ for example to watch how church numerals could be converted back to normal ones. let $s=\lambda x.(x+1), z=0$, then:

$$
\begin{array}{}
2sz&=&(\lambda s.\lambda z.s(s(z)))sz\\
&=&s(s(z))\\
&=&s(s(0))\\
&=&s(0+1)\\
&=&1+1\\
&=&2\\
\end{array}
$$

It is clear now: $s$ stands for succussor and $z$ stands for zero. It is built base on recursion. And yes, it is exactly how natural numbers are defined mathematically.

## Successor

To get the successor of a church numeral, just simply wrap an $s$ around it.

$$
S=\lambda n.\lambda s.\lambda z.(s(nsz))\\
Sn=n+1
$$

Proof:

$$
\begin{array}{}
Sn&=&(\lambda n.\lambda s.\lambda z.(s(nsz)))(\lambda s.\lambda z.s^n(z))\\
&=&(\lambda s'.\lambda z'.(s'((\lambda s.\lambda z.s^n(z))s'z')))\\
&=&(\lambda s'.\lambda z'.(s'(s'^n(z'))))\\
&=&(\lambda s'.\lambda z'.(s'^{n+1}(z')))\\
&=&(\lambda s.\lambda z.(s^{n+1}(z)))\\
&=&n+1\\
\end{array}
$$

## Addition

A Church numeral $n$ is actually a recursion builder repeating a function for $n$ times. Making use of this the addition operation of church numerals could be deduced.

$$
\text{add}=\lambda mn.(mSn)\\
\text{add }mn=m+n
$$

It reads as if "evaluating $m^\text{th}$ successor of $n$". 

Proof:

$$
\begin{array}{}
\text{add }mn&=&(\lambda mn.(mSn))mn\\
&=&(\lambda s.\lambda z.s^m(z))S(\lambda s.\lambda z.s^n(z))\\
&=&\lambda z.S^m(z)(\lambda s.\lambda z.s^n(z))\\
&=&S^m(\lambda s.\lambda z.s^n(z))\\
&=&\lambda s.\lambda z.s^{m+n}(z)\\
&=&m+n\\
\end{array}
$$

Actually, there is a direct definition of addition.

$$
\text{add}=\lambda m.\lambda n.\lambda s.\lambda z.ms(nsz)\\
$$

It reads as if "evaluating $m^\text{th}$ successor of '$n^\text{th}$ successor of $0$'". 

Proof is similar to indirect one.

## Multiplication

Indirect definition:

$$
\text{mul}=\lambda mn.m(\text{add }n)0\\
\text{mul }mn=m\times n
$$

It reads as if "add $n$ for $m$ times to $0$".

Direct definition:

$$
\text{mul}=\lambda m.\lambda n.\lambda s.\lambda z.m(ns)z
$$

It reads as if "'evaluating $n^\text{th}$ successor' for $m$ times of $0$".

Proofs are similar to the addition operation.

## Exponentiation

Indirect definition:

$$
\text{exp}=\lambda mn.n(\text{mul }m)1\\
\text{exp }mn=m^n 
$$

It reads as if "multiplies $m$ for $n$ times to $1$".

Proof is similar to the multiplication operation.

Direct definition:

$$
\text{exp}=\lambda m.\lambda n.\lambda s.\lambda z.nm(sz)
$$

It could hardly read as if a statement, but proof may help you understand.

Proof:

$$
\begin{array}{}
\text{exp }mn=\lambda s.\lambda z.nm(sz)&=&(\lambda sz.s^n(z))(\lambda sz.s^m(z))(sz)\\
&=&(\lambda sz.s^m(z))^n(sz)&=&(\lambda sz.s^m(z))^n(1)\\
\text{(add } 1\text{ for } m \text{ times to 0)}&=&(\lambda sz.s^m(z))^{n-1}(\lambda z.mz)&=&(\lambda sz.s^m(z))^{n-1}(m)\\
\text{(add } m\text{ for } m \text{ times to 0)}&=&(\lambda sz.s^m(z))^{n-2}(\lambda z.m^2z)&=&(\lambda sz.s^m(z))^{n-2}(m^2)\\
\text{(add } m^2\text{ for } m \text{ times to 0)}&=&(\lambda sz.s^m(z))^{n-3}(\lambda z.m^3z)&=&(\lambda sz.s^m(z))^{n-3}(m^3)\\
&&\cdots\\
&=&(\lambda sz.s^m(z))(\lambda z.m^{n-1}z)&=&(\lambda sz.s^m(z))(m^{n-1})\\
\text{(add } m^{n-1}\text{ for } m \text{ times to 0)}&=&\lambda z.m^nz&=&m^n\\
\end{array}
$$

## Sequences

Observe the architecture of sequences and church numerals:

$$
\begin{array}{l}
&\text{Sequences}&\text{Church Numerals}\\
\text{Initial term}&a_0 & z\\
\text{Recurrence function}&f_{a_{n-1}\rightarrow a_n} & s
\end{array}
$$

And yes, natural numbers, are no more than a special arithmetic sequence with initial $0$ and successor fucntion $\lambda x.(x+1)$. 

Church numerals, however, are unnecessary to be mere natural numbers, not even mere arithmetic sequence, but whatever sequence you want! e. g. 

- $s=\lambda x.(x+d), z=a_0$ makes a arithmetic sequence.
- $s=\lambda x.(x\times q), z=a_0 (q\ne0)$ makes a geometric sequence.

Let's prove obscure direct definition of exponentiation via geometric sequence:

$$
\text{exp }mn=\lambda s.\lambda z.ns'z'=m^n
$$

$s'$ should be a multiplier of $m$, so it should evaluate $m^{\text{th}}$ succussor to $0$, regardless of succussor function, which represents previous result of evaluation.

$$
\begin{array}{}
s'&=&\lambda x.\lambda z.(m\times x+z)\\
&=&\lambda x.\lambda z.(\underbrace{x+x+\cdots+x}_{m \text{ times}}+z)\\
&=&\lambda s.\lambda z.s^m(z)\\
&=&m
\end{array}
$$

$z'$ should be one. 

$$
z'=sz
$$

Neat.